More proof

inductive_proof/Queue_merge_list/App.fst
@@ -484,7 +484,7 @@ let rec lem_s1s2_then_lca (lca s1 s2:st)
               assert (not (L.mem (fst last1, get_ele last1) (v_of lca)));
               ()))
 
-let common (lca s1 s2:st)
+(*let common (lca s1 s2:st)
   : Lemma (requires consistent_branches lca s1 s2 /\
                     sorted (v_of lca) /\ sorted (v_of s1) /\ sorted (v_of s2))
           (ensures (let i = intersection (v_of lca) (v_of s1) (v_of s2) in
@@ -497,7 +497,7 @@ let common (lca s1 s2:st)
                     (forall id. mem_id_s id i ==> (not (mem_id_s id da) /\ not (mem_id_s id db))) /\
                     (forall id id1. mem_id_s id (v_of lca) /\ mem_id_s id1 da ==> id < id1) /\
                     (forall id id1. mem_id_s id (v_of lca) /\ mem_id_s id1 db ==> id < id1) /\
-                    (forall id. mem_id_s id da ==> not (mem_id_s id db)))) = admit()
+                    (forall id. mem_id_s id da ==> not (mem_id_s id db)))) = admit()*)
 
 let rec lem_inter (l a b:concrete_st)
   : Lemma (requires (forall e. (L.mem e a /\ L.mem e b) ==> L.mem e l) /\
@@ -519,7 +519,7 @@ let help (p s h xs hd:concrete_st)
     L.append_assoc p h s;
     L.append_assoc hd (L.append p h) s
 
-let rec intersectionLemma1 (l a b: concrete_st)
+(*let rec intersectionLemma1 (l a b: concrete_st)
   : Lemma (requires (forall e. (L.mem e a /\ L.mem e b) ==> L.mem e l) /\
                     sorted l /\ sorted a /\ sorted b /\
                     a <> [] /\ b <> [] /\ L.hd a = L.hd b)
@@ -535,7 +535,7 @@ let rec intersectionLemma1 (l a b: concrete_st)
                               L.append_assoc [] [L.hd a] xs;
                               assert (exists p s. xs == L.append (L.append p [L.hd a]) s);
                               assume (exists p s. L.append [x] xs == L.append (L.append (L.append [x] p) [L.hd a]) s); //todo
-                              ()) else ())
+                              ()) else ())*)
 
 let rec inter (l a' b' a b: concrete_st)
   : Lemma (requires (forall e. (L.mem e a' /\ L.mem e b') ==> L.mem e l) /\
@@ -552,17 +552,17 @@ let rec inter (l a' b' a b: concrete_st)
                     else (assert (x <> y /\ x <> z);
                           if y = z then (inter xs a' b' a b) else ())
                           
-let rec diff_lem (l a' a: concrete_st)
-  : Lemma (requires sorted l /\ sorted a /\ sorted a' /\
-                    a' <> [] /\ a = L.tl a')
-          (ensures (let da' = diff_s l a' in
-                    let da = diff_s l a in
-                    da' = da)) =
+let rec diff_lem (a' l: concrete_st)
+  : Lemma (requires sorted l /\ sorted a' /\
+                    a' <> [] /\ L.mem (L.hd a') l)
+          (ensures (let da' = diff_s a' l in
+                    let da = diff_s (L.tl a') l in
+                    da' = da))
+          (decreases %[a';l]) =
   match a', l with
   |[],_ -> ()
   |_,[] -> ()
-  |x::xs,y::ys -> if x <> y then (admit(); diff_lem a' ys a)
-               else if xs <> [] then (admit();diff_lem xs ys (L.tl xs)) else admit()
+  |x::xs,y::ys -> if x <> y then diff_lem a' ys else ()
                           
 #push-options "--z3rlimit 100"
 let lin_gt0_s1's2'_dd_eq' (lca s1 s2:st) (last1 last2:op_t)
@@ -591,7 +591,6 @@ let lin_gt0_s1's2'_dd_eq' (lca s1 s2:st) (last1 last2:op_t)
      assume (sorted (v_of lca) /\ sorted (v_of s1) /\ sorted (v_of s2)); //todo
      lem_s1s2_then_lca lca s1 s2;
      lem_inter (v_of lca) (v_of s1) (v_of s2);
-     intersectionLemma1 (v_of lca) (v_of s1) (v_of s2);
      let i' = intersection (v_of lca) (v_of s1) (v_of s2) in
      let i = intersection (v_of lca) (do (v_of s1) last1) (do (v_of s2) last2) in
      let da' = diff_s (v_of s1) (v_of lca) in
@@ -602,7 +601,9 @@ let lin_gt0_s1's2'_dd_eq' (lca s1 s2:st) (last1 last2:op_t)
      assert (do (v_of s1) last1 == L.tl (v_of s1) /\ do (v_of s2) last2 == L.tl (v_of s2));
      inter (v_of lca) (v_of s1) (v_of s2) (do (v_of s1) last1) (do (v_of s2) last2);
      assert (L.tl i' = i); 
-     assume (da = da' /\ db = db');
+     diff_lem (v_of s1) (v_of lca);
+     diff_lem (v_of s2) (v_of lca);
+     assert (da = da' /\ db = db');
      ())
 
 let lin_gt0_s1's2'_trial (lca s1 s2:st)
